Test/git-issues/git-issue-3804.dfy
@@ -6,7 +6,7 @@ predicate P(x: int)
 function FirstAssertNotProved(): (i: int)
   ensures P(i)
 {
-  assert rule2: P(12) by {
+  assert rule2: P(12) by { // error: cannot be verified here
   }
   assert P(12) by {
     reveal rule2;
@@ -17,9 +17,9 @@ function FirstAssertNotProved(): (i: int)
 function BothAssertNotProved(): (i: int)
   ensures P(i)
 {
-  assert rule2: P(12) by {
+  assert rule2: P(12) by { // error: cannot be verified here
   }
-  assert P(12) by { // Fails
+  assert P(12) by { // error: cannot be verified here
   }
   12
 }
@@ -28,7 +28,7 @@ function FirstAssertNotProvedBecauseRequiresNotRevealed(): (i: int)
   requires rule: P(12)
   ensures P(i)
 {
-  assert rule2: P(12) by {
+  assert rule2: P(12) by { // error: cannot be verified here
   }
   assert P(12) by {
     reveal rule2;
@@ -45,7 +45,7 @@ function SecondAssertNotProvedBecauseAssertNotRevealed(): (i: int)
   assert rule2: P(12) by {
     reveal rule;
   }
-  assert P(12) by {
+  assert P(12) by { // error: cannot be verified here
   }
   12
 }
@@ -61,4 +61,21 @@ function EverythingVerifies(): (i: int)
     reveal rule2;
   }
   12
+}
+
+least predicate ShouldNotWork(): (y: bool)
+  requires rule: P(12)
+{
+  assert P(12) by { // Error, cannot prove this
+  }
+  true
+}
+
+least predicate ShouldWork(): (y: bool)
+  requires rule: P(12)
+{
+  assert P(12) by {
+    reveal rule;
+  }
+  true
 }
